trying to prove termination mgu

mgu.fst
@@ -2,7 +2,7 @@ module Mgu
 
 open Term
 open Subst
-open FStar.Set
+open FSet
 open Union
 
 val apply_tuple_list : st:subst -> l:list (term*term) -> Tot (list (term*term))
@@ -44,20 +44,16 @@ and get_list_of_vars_list lt lv = match lt with
                 get_list_of_vars_list tl temp1
               end*)
 
-val get_num_vars : term -> set variable -> Tot (nat*(set variable))
-val get_num_vars_list : list term -> set variable  -> Tot (nat*(set variable))
+val get_fset_vars : term -> Tot fset
+val get_fset_vars_list : list term -> Tot fset
 
-let rec get_num_vars t sv = match t with
-  | Var v -> if mem v sv then (0,sv) else  (1,(union sv (singleton v)))
-  | Name n -> (0,sv)
-  | Func s args -> get_num_vars_list args sv
-and get_num_vars_list lt sv = match lt with
-  | [] -> (0,empty)
-  | hd::tl -> begin
-              let temp1 = get_num_vars hd sv in
-              let temp2 = (get_num_vars_list tl (snd temp1)) in
-              ((fst temp1)+(fst temp2),(snd temp2))
-              end
+let rec get_fset_vars t= match t with
+  | Var v -> fsingleton v
+  | Name n -> fempty
+  | Func s args -> get_fset_vars_list args sv
+and get_fset_vars_list lt = match lt with
+  | [] -> fempty
+  | hd::tl -> funion (get_fset_vars hd) (get_fset_vars_list tl)
 
 val get_num_symbols : t:term -> Tot nat
 val get_num_symbols_list : lt:list term-> Tot nat
@@ -71,58 +67,21 @@ and get_num_symbols_list lt = match lt with
   | [] -> 0
   | hd::tl -> get_num_symbols hd + get_num_symbols_list tl
 
-val get_num_vars_tuple_list : list (term*term) -> set variable -> Tot nat
+val get_fset_vars_tuple_list : list (term*term) -> Tot fset
 
-let rec get_num_vars_tuple_list ltt sv = match ltt with
-  | [] -> 0
-  | (hd1,hd2)::tl -> let temp1 = get_num_vars hd1 sv in
-                    let temp2 = get_num_vars hd2 (snd temp1) in
-                    (fst temp1) + (fst temp2) + (get_num_vars_tuple_list tl (snd temp2))
+let rec get_fset_vars_tuple_list ltt = match ltt with
+  | [] -> empty
+  | (hd1,hd2)::tl -> union (get_fset_vars hd1)  (union (get_fset_vars hd2) (get_fset_vars_tuple_list tl))
 
-val rearrange_tuple_list : #a:eqtype -> list(a*a) -> Tot (list a)
+val aux_lemma1 : ltt:list (term*term) -> t:term -> v:variable -> Lemma
+  (requires not(is_var_present v x))
+  (ensures fsubset (get_fset_vars_tuple_list (apply_tuple_list [(v,t)] ltt)) (get_fset_vars_tuple_list ( (Var v,t)::ltt ) ) &&
+          fsubset (get_fset_vars_tuple_list (apply_tuple_list [(v,t)] ltt)) (get_fset_vars_tuple_list ( (t,Var v)::ltt ) ) )
 
-let rec rearrange_tuple_list #a l = match l with
-  | [] -> []
-  | (x,y)::tl -> x::(y::(rearrange_tuple_list tl))
+val aux_lemma2 : 
 
 
-val aux_lemma1a : t:term -> sv1:set variable -> sv2:set variable -> Lemma (requires true) (ensures (subset sv1 sv2  ==> (fst (get_num_vars t sv1) >= fst (get_num_vars t sv2))))
-val aux_lemma1b : lt:list term -> sv1:set variable -> sv2:set variable -> Lemma
-  (requires subset sv1 sv2)
-  (ensures (fst (get_num_vars_list lt sv1) >= fst (get_num_vars_list lt sv2)))
-val aux_lemma1e : t:term -> sv:set variable -> Lemma (requires true)(ensures (subset (sv) (snd (get_num_vars t sv))))
-val aux_lemma1f : lt:list term -> sv:set variable -> Lemma (requires true)(ensures (subset (sv) (snd (get_num_vars_list lt sv))))
-let rec aux_lemma1e t sv = match t with
-  | Var v -> ()
-  | Name n -> ()
-  | Func s args -> aux_lemma1f args sv
-and aux_lemma1f lt sv = match lt with
-  | [] -> ()
-  | hd::tl -> aux_lemma1e hd sv
-
-let rec aux_lemma1a t sv1 sv2 = match t with
-  | Var v -> if mem v sv1 then (assert (fst (get_num_vars t sv1) = 0); assert (fst (get_num_vars t sv2) = 0))
-             else if mem v sv2 then (assert (fst (get_num_vars t sv1) = 1); assert (fst (get_num_vars t sv2) = 0))
-             else (assert (fst (get_num_vars t sv1) = 1); assert (fst (get_num_vars t sv2) = 1))
-  | Name n -> (assert (fst (get_num_vars t sv1) = 0); assert (fst (get_num_vars t sv2) = 0))
-  | Func s args -> aux_lemma1b args sv1 sv2
-and aux_lemma1b lt sv1 sv2 = match lt with
-  | [] -> ()
-  | hd::tl -> aux_lemma1a hd sv1 sv2 ;aux_lemma1b tl sv1 sv2
-
-val aux_lemma2 : hd1:term -> hd2:term -> tl:list (term*term) -> Lemma
-  (requires true)
-  (ensures get_num_vars_tuple_list ((hd1,hd2)::tl) empty <= fst (get_num_vars hd1 empty) + fst (get_num_vars hd2 empty) + get_num_vars_tuple_list tl empty)
-
-let aux_lemma2 hd1 hd2 tl= ()
-
-val aux_lemma9 : v:variable -> x:term -> ltt:list (term*term) -> Lemma
-  (requires true)
-  (ensures get_num_vars_tuple_list (apply_tuple_list [(v,x)] ltt) empty < get_num_vars_tuple_list ((Var v,x)::ltt) empty)
-
-let rec aux_lemma9 v x ltt = admit()
-
-val sub_mgu : l:list (term*term) -> st:subst -> Tot (option subst) (decreases %[get_num_vars_tuple_list l empty;(get_num_symbols_list (rearrange_tuple_list l))])
+val sub_mgu : l:list (term*term) -> st:subst -> Tot (option subst) (decreases %[size (get_fset_vars_tuple_list l);(get_num_symbols_list (rearrange_tuple_list l))])
 let rec sub_mgu l st = match l with
   | [] -> Some st
   | (Var v, x)::tl
